WIP: Executability

Ground_PDDL_Exec_Imp/Ground_PDDL_NTA_Reduction_Impl.thy
@@ -6,7 +6,59 @@ begin
 
 lemmas return_iff = return_iff check_all_list_return_iff check_wf_problem_return_iff
 
-named_theorems return_if
+lemma context_bind_return_iff[return_iff]:
+  "(m \<bind> f = Inr y) = (\<exists>x. m = Inr x \<and> (m = Inr x \<longrightarrow> f x = Inr y))"
+  apply (subst return_iff)
+  by auto
+
+lemma context_bind_return_iff'[return_iff]:
+  "(m \<bind> f = Inr y) = (\<exists>x P. m = Inr x \<and> (m = Inr x \<longleftrightarrow> P) \<and> (P \<longrightarrow> f x = Inr y))"
+  apply (subst context_bind_return_iff)
+  by simp
+
+lemma mapM_return_iff[return_iff]: "mapM f xs = Inr ys \<longleftrightarrow> list_all2 (\<lambda>x y. f x = Inr y) xs ys"
+proof (rule iffI)
+  assume a: "mapM f xs = Inr ys"
+  have len: "length xs = length ys" using a mapM_return by fastforce
+  show "list_all2 (\<lambda>x y. f x = Inr y) xs ys"
+  proof (rule list_all2_all_nthI[OF len])
+    fix n
+    assume n: "n < length xs" 
+    have ys: "ys = map (projr \<circ> f) xs" 
+      and xs_r: "(\<forall>x\<in>set xs. \<forall>e. f x \<noteq> Inl e)" using a[THEN mapM_return] by blast+
+    obtain r where
+        xs_n_inr: "f (xs ! n) = Inr r" using xs_r n apply (cases "f (xs ! n)") by auto
+    have "ys ! n = r" using xs_n_inr ys unfolding comp_def using n by simp
+    thus "f (xs ! n) = Inr (ys ! n)" using xs_n_inr by simp
+  qed
+next
+  assume a: "list_all2 (\<lambda>x y. f x = Inr y) xs ys"
+  thus "mapM f xs = Inr ys"
+    by (induction rule: list_all2_induct) auto
+qed
+
+
+lemma list_all2_return_if:
+  assumes "list_all P xs"
+      and "\<And>x y. P x \<Longrightarrow> fM x = Inr y \<longleftrightarrow> f x = y"
+    shows "list_all2 (\<lambda>x y. fM x = Inr y) xs ys = (ys = map f xs)"
+  unfolding list_all2_conv_all_nth
+proof (intro iffI strip conjI; (elim conjE)?)
+  assume len: "length xs = length ys" 
+    and i: "\<forall>i<length xs. fM (xs ! i) = Inr (ys ! i)"
+  have nth_eq: "\<forall>i < length xs. ys ! i = f (xs ! i)" using i assms unfolding list_all_iff by simp
+  show "ys = map f xs" apply (subst list_eq_iff_nth_eq)
+    using len nth_eq by auto 
+next
+  show "ys = map f xs \<Longrightarrow> length xs = length ys" by simp
+next
+  fix i
+  assume ys: "ys = map f xs"
+    and i: "i < length xs"
+  show "fM (xs ! i) = Inr (ys ! i)"
+    using assms ys i unfolding list_all_iff by auto
+qed
+
 
 definition "example_domain =
 Domain [] [] [] [] []
@@ -50,22 +102,538 @@ proof -
     by (force simp: wf_problem'_correct return_iff)
 qed
 
-value "check_ground_problem example_problem"
 
-lemma context_bind_return_iff[return_iff]:
-  "(m \<bind> f = Inr y) = (\<exists>x. m = Inr x \<and> (m = Inr x \<longrightarrow> f x = Inr y))"
-  apply (subst return_iff)
-  by auto
+definition "prop_to_var_impl prop_to_name p \<equiv> STR ''var_'' + prop_to_name p"
+definition "prop_to_lock_impl prop_to_name p \<equiv> STR ''lock_'' + prop_to_name p"
+definition "acts_active_impl \<equiv> STR ''acts_active''"
+definition "planning_lock_impl \<equiv> STR ''planning_lock''"
 
-lemma context_bind_return_iff'[return_iff]:
-  "(m \<bind> f = Inr y) = (\<exists>x P. m = Inr x \<and> (m = Inr x \<longleftrightarrow> P) \<and> (P \<longrightarrow> f x = Inr y))"
-  apply (subst context_bind_return_iff)
-  by simp
+definition "act_to_start_clock_impl act_to_name a \<equiv> STR ''start_'' + act_to_name a"
+definition "act_to_end_clock_impl act_to_name a \<equiv> STR ''end_'' + act_to_name a"
+definition "urge_clock_impl \<equiv> STR ''urge_clock''"
+
+definition "off_loc_impl \<equiv> 0::nat"
+definition "starting_loc_impl \<equiv> 1::nat"
+definition "running_loc_impl \<equiv> 2::nat"
+definition "ending_loc_impl \<equiv> 3::nat"
+
+definition "init_loc_impl \<equiv> 0::nat"
+definition "planning_loc_impl \<equiv> 1::nat"
+definition "goal_loc_impl \<equiv> 2::nat"
+
+abbreviation "var_is n v \<equiv> bexp.eq (exp.var v) (exp.const n)"
+abbreviation "inc_var n v \<equiv> (v, exp.binop (+) (exp.var v) (exp.const n))"
+abbreviation "set_var n v \<equiv> (v, exp.const n)"
+
+
+fun lower_spec_impl::"ast_action_schema \<Rightarrow> _" where
+"lower_spec_impl (Simple_Action_Schema n ps pre eff) = Some (lower_bound.GE 0)" | (* could also be None *)
+"lower_spec_impl (Durative_Action_Schema n ps d cond eff) = map_option (map_lower_bound floor) (dc_list_lower d)"
+
+fun upper_spec_impl::"ast_action_schema \<Rightarrow> _" where
+"upper_spec_impl (Simple_Action_Schema n ps pre eff) = Some (upper_bound.LE 0)" | (* could also be None *)
+"upper_spec_impl (Durative_Action_Schema n ps d cond eff) = map_option (map_upper_bound floor) (dc_list_upper d)"
+
+definition "l_dur_spec_impl a \<equiv> (case lower_spec_impl a of 
+  None \<Rightarrow> [] | Some (lower_bound.GT n) \<Rightarrow> 
+    [acconstraint.GT (act_to_start_clock_impl ast_action_schema.name a) n]
+| Some (lower_bound.GE n) \<Rightarrow> 
+    [acconstraint.GE (act_to_start_clock_impl ast_action_schema.name a) n])"
+
+
+definition "u_dur_spec_impl a \<equiv> (case upper_spec_impl a of 
+  None \<Rightarrow> [] | Some (upper_bound.LT n) \<Rightarrow> 
+    [acconstraint.LT (act_to_start_clock_impl ast_action_schema.name a) n]
+| Some (upper_bound.LE n) \<Rightarrow> 
+    [acconstraint.LE (act_to_start_clock_impl ast_action_schema.name a) n])"
+
+definition main_auto_loop_spec_impl::"(nat \<times>
+    (String.literal, int) Simple_Expressions.bexp \<times>
+    (String.literal, int) acconstraint list \<times>
+    String.literal act \<times>
+    (String.literal \<times> (String.literal, int) exp) list \<times>
+    String.literal list \<times> nat)" where
+"main_auto_loop_spec_impl \<equiv> (goal_loc_impl, bexp.true, [], Sil STR '''', [], [], goal_loc_impl)"
+
+
+context ground_ast_problem_defs
+begin
+
+text \<open>We define the code that generates the automata\<close>
+
+definition "mutex_snap_action' a b = 
+  action_defs.mutex_snap_action (\<lambda>a. set (imp_defs.rat_impl.pre_imp_list a)) (\<lambda>a. set (imp_defs.rat_impl.add_imp_list a)) (\<lambda>a. set (imp_defs.rat_impl.del_imp_list a)) a b"
+
+definition "int_clocks_spec' a =
+    map (act_to_start_clock_impl ast_action_schema.name) (filter (\<lambda>b. mutex_snap_action' a (AtStart b)) actions_spec) 
+  @ map (act_to_end_clock_impl ast_action_schema.name) (filter (\<lambda>aa. mutex_snap_action' a (AtEnd aa)) actions_spec)"
+
+definition "start_edge_spec' a = 
+(let start_snap = AtStart a; guard = map (\<lambda>x. acconstraint.GT x 0) (int_clocks_spec' start_snap) @ map (\<lambda>x. acconstraint.GE x 0) (int_clocks_spec' start_snap);
+  not_locked_check = map ((var_is 0 \<circ>\<circ> prop_to_lock_impl) predicate.name) (filter (\<lambda>p. p \<notin> set (imp_defs.rat_impl.add_imp_list start_snap)) (imp_defs.rat_impl.del_imp_list start_snap)); 
+  pre_check = map ((var_is 1 \<circ>\<circ> prop_to_var_impl) predicate.name) (imp_defs.rat_impl.pre_imp_list start_snap);
+  var_check = bexp_and_all (not_locked_check @ pre_check); 
+  add_upds = map ((set_var 1 \<circ>\<circ> prop_to_var_impl) predicate.name) (imp_defs.rat_impl.add_imp_list start_snap); 
+  del_upds = map ((set_var 0 \<circ>\<circ> prop_to_var_impl) predicate.name) (imp_defs.rat_impl.del_imp_list start_snap);
+  upds = (inc_var 1 acts_active_impl) # del_upds @ add_upds; 
+  resets = [act_to_start_clock_impl ast_action_schema.name a]
+ in (off_loc_impl, var_check, guard, Sil STR '''', upds, resets, starting_loc_impl))"
+
+definition "edge_2_spec' a =
+(let 
+  check_invs = bexp_and_all (map ((var_is 1 \<circ>\<circ> prop_to_var_impl) predicate.name) (over_all_spec a));
+  upds = map ((inc_var 1 \<circ>\<circ> prop_to_lock_impl) predicate.name) (over_all_spec a)
+in (starting_loc_impl, check_invs, [], Sil STR '''', upds, [], running_loc_impl))"
+
+definition "edge_3_spec' a =
+(let 
+  end_snap = AtEnd a; 
+  int_clocks = map (\<lambda>x. acconstraint.GT x 0) (int_clocks_spec' end_snap) @ map (\<lambda>x. acconstraint.GE x 0) (int_clocks_spec' end_snap); 
+  guard = l_dur_spec_impl a @ u_dur_spec_impl a @ int_clocks;
+  upds = map ((inc_var (- 1) \<circ>\<circ> prop_to_lock_impl) predicate.name) (over_all_spec a); 
+  resets = [act_to_end_clock_impl ast_action_schema.name a]
+in (running_loc_impl, bexp.true, guard, Sil STR '''', upds, resets, ending_loc_impl))"
+
+definition "end_edge_spec' a =
+(let 
+  end_instant = ending_loc_impl; 
+  off = off_loc_impl; 
+  end_snap = AtEnd a; 
+  not_locked_check = map ((var_is 0 \<circ>\<circ> prop_to_lock_impl) predicate.name) (filter (\<lambda>p. p \<notin> set (imp_defs.rat_impl.add_imp_list end_snap)) (imp_defs.rat_impl.del_imp_list end_snap));
+  pre_check = map ((var_is 1 \<circ>\<circ> prop_to_var_impl) predicate.name) (imp_defs.rat_impl.pre_imp_list end_snap); 
+  check = bexp_and_all (not_locked_check @ pre_check);
+  add_upds = map ((set_var 1 \<circ>\<circ> prop_to_var_impl) predicate.name) (imp_defs.rat_impl.add_imp_list end_snap); 
+  del_upds = map ((set_var 0 \<circ>\<circ> prop_to_var_impl) predicate.name) (imp_defs.rat_impl.del_imp_list end_snap);
+  upds = inc_var (- 1) acts_active_impl # del_upds @ add_upds
+in (end_instant, check, [], Sil STR '''', upds, [], off))"
+
+
+definition "instant_trans_edge_spec' a =
+(let 
+  end_snap = AtEnd a; 
+  start_snap = AtStart a; 
+  int_clocks = map (\<lambda>x. acconstraint.GT x 0) (int_clocks_spec' end_snap) @ map (\<lambda>x. acconstraint.GE x 0) (int_clocks_spec' end_snap); 
+  guard = l_dur_spec_impl a @ u_dur_spec_impl a @ int_clocks;
+ resets = [act_to_end_clock_impl ast_action_schema.name a]
+in (starting_loc_impl, bexp.true, guard, Sil STR '''', [], resets, ending_loc_impl))"
+
+
+definition "action_to_automaton_spec' a =
+(let committed_locs = []; 
+  urgent_locs = [starting_loc_impl, ending_loc_impl]; 
+  edges = [start_edge_spec' a, edge_2_spec' a, edge_3_spec' a, end_edge_spec' a, instant_trans_edge_spec' a];
+  invs = []
+in (committed_locs, urgent_locs, edges, invs))"
+
+text \<open>We do the same for the main automaton\<close>
+
+definition "init_spec' = (map to_predicate (filter is_predAtom (init P)))"
+
+definition "main_auto_init_edge_spec' \<equiv>
+(let can_start = var_is 0 planning_lock_impl;
+  permit_planning = set_var 1 planning_lock_impl; 
+  set_active = set_var 0 acts_active_impl;
+  set_props = map ((set_var 1 \<circ>\<circ> prop_to_var_impl) predicate.name) init_spec'; 
+  upds = permit_planning # set_active # set_props
+in (init_loc_impl, can_start, [], Sil STR '''', upds, [], planning_loc_impl))
+"
+
+definition main_auto_goal_edge_spec'::"nat \<times>
+   (String.literal, int) Simple_Expressions.bexp \<times>
+   (String.literal, int) acconstraint list \<times>
+   String.literal act \<times>
+   (String.literal \<times> (String.literal, int) exp) list \<times> String.literal list \<times> nat" where
+"main_auto_goal_edge_spec' \<equiv>
+(let 
+  can_end = [var_is 1 planning_lock_impl, var_is 0 acts_active_impl]; 
+  goal_sat = map ((var_is 1 \<circ>\<circ> prop_to_var_impl) predicate.name) goal_spec;
+  cond = bexp_and_all (can_end @ goal_sat); 
+  lock_plan = (planning_lock_impl, exp.const 2)
+in (planning_loc_impl, cond, [], Sil STR '''', [lock_plan], [], goal_loc_impl))
+"
+
+definition main_auto_spec'::"nat list \<times>
+   nat list \<times>
+   (nat \<times>
+    (String.literal, int) Simple_Expressions.bexp \<times>
+    (String.literal, int) acconstraint list \<times>
+    String.literal act \<times>
+    (String.literal \<times> (String.literal, int) exp) list \<times>
+    String.literal list \<times> nat) list \<times>
+   (nat \<times> (String.literal, int) acconstraint list) list" where
+"main_auto_spec' \<equiv>
+(let committed_locs = []; 
+  urgent_locs = [init_loc_impl, goal_loc_impl]; 
+  edges = [main_auto_init_edge_spec', main_auto_goal_edge_spec', main_auto_loop_spec_impl]; 
+  invs = [] 
+in (committed_locs, urgent_locs, edges, invs))"
+
+definition "automata_spec' = main_auto_spec' # map action_to_automaton_spec' actions_spec"
+
+end
+
+
+find_theorems "finite ?x \<Longrightarrow> inj ?f \<Longrightarrow> finite ?y"
+find_theorems name: "infinite*UNIV"
+
+lemma UNIV_predicate:
+  "(UNIV::predicate set) = Pred ` (UNIV::String.literal set)"
+  apply (intro equalityI subsetI UNIV_I)
+  subgoal for x
+    unfolding UNIV_def 
+    apply (cases x)
+    by blast
+  done
+
+lemma inifinite_UNIV_literalI:
+  "infinite (UNIV::String.literal set)"
+proof (rule notI)
+  assume "finite (UNIV::String.literal set)"
+  moreover
+  have "inj (\<lambda>l::String.literal. (STR ''x'') + l)"
+    apply (rule injI)
+    apply (subst (asm) String.add_literal_code)+
+    using String.Literal_eq_iff by simp
+  ultimately
+  have "surj (\<lambda>l::String.literal. (STR ''x'') + l)"
+    using finite_UNIV_inj_surj by blast
+  then obtain s where "STR '''' = STR ''x'' + s" by (rule surjE)
+  thus False by (simp add: String.add_literal_code String.Literal_eq_iff)
+qed
+
+
+find_theorems "infinite (?f ` ?x)"
+
+lemma range_inj_infinite:
+  assumes "infinite S"
+      and "inj f"
+    shows "infinite (f ` S)"
+proof
+  assume a: "finite (f ` S)"
+  have "f -` (f ` S) = S" using \<open>inj f\<close> inj_vimage_image_eq by simp
+  moreover
+  have "finite (f -` (f ` S))" using finite_vimageI a \<open>inj f\<close> by blast
+  ultimately
+  have "finite S" by auto
+  with \<open>infinite S\<close>
+  show False by simp
+qed
+
+lemma infinite_UNIV_predicateI:
+  "infinite (UNIV::predicate set)"
+  apply (subst UNIV_predicate)
+  apply (rule range_inj_infinite)
+   apply (rule inifinite_UNIV_literalI)
+  apply (rule injI)
+  by blast
+
+instantiation predicate :: card_UNIV
+begin 
+definition "finite_UNIV = Phantom(predicate) False"
+definition "card_UNIV = Phantom(predicate) 0"
+instance by intro_classes (simp_all add: finite_UNIV_predicate_def card_UNIV card_UNIV_predicate_def infinite_UNIV_predicateI)
+end
+
+find_theorems name: "proper_int*char"
+
+find_theorems name: "ord*list"
+
+find_theorems name: "less*liter"
+
+find_theorems "List.ord.lexordp"
+
+instantiation String.literal :: proper_interval
+begin
+value "String.digit7 (Char True True True True True True True False)"
+value "String.ascii_of (Char True True True True True True True False)"
+
+fun char_less_one::"char \<Rightarrow> char \<Rightarrow> bool"where
+"char_less_one c d = (of_char d - of_char c > (0::nat))"
+
+fun list_less_one::"char list \<Rightarrow> char list \<Rightarrow> bool" where
+"list_less_one _ [] = False" |
+"list_less_one [] (y#ys) = (char_less_one (CHR 0x00) y \<or> length ys > 0)" |
+"list_less_one [x] (y#ys) = (char_less_one x (CHR 0x7F) \<or> list_less_one [] ys)" |
+"list_less_one (x#xs) (y#ys) = (char_less_one x y \<or> list_less_one xs ys)"
+
+
+fun proper_interval_literal::"String.literal option \<Rightarrow> String.literal option \<Rightarrow> bool" where
+"proper_interval_literal None None = True" |
+"proper_interval_literal (Some s) None = True" |
+"proper_interval_literal None (Some s) = (s \<noteq> (STR ''''))" |
+"proper_interval_literal (Some s) (Some t) = (list_less_one (literal.explode s) (literal.explode t))"
+
+instance 
+proof
+  show "proper_interval None (None::String.literal option) = True" by simp
+  show "\<And>y::String.literal. proper_interval None (Some y) = (\<exists>z. z < y)"
+  proof
+    fix y::"String.literal"
+    assume "proper_interval None (Some y)"
+    hence yn: "y \<noteq> STR ''''" by simp
+    hence "literal.explode y \<noteq> []" 
+      using literal.explode_inject zero_literal.rep_eq by metis
+    then obtain c cs where
+      xy: "literal.explode y = c # cs" apply (cases "literal.explode y") by simp+
+    have "STR '''' < y" using xy zero_literal.rep_eq 
+      apply (subst less_literal.rep_eq) by auto
+    thus "\<exists>z. z < y" by fast
+  next
+    fix y::"String.literal"
+    assume "\<exists>z. z < y"
+    then obtain z where
+      le: "z < y" by blast
+    {
+      assume "y = (STR '''')"
+      hence "y \<le> z"
+        apply (cases "literal.explode z")
+        using zero_literal.rep_eq
+        using less_eq_literal.rep_eq
+        by auto
+      hence False using le by force
+    }
+    thus "proper_interval None (Some y)" by auto
+  qed
+  show "\<And>x::String.literal. proper_interval (Some x) None = (\<exists>z. x < z)" 
+  proof -
+    fix x::"String.literal"
+    { have "literal.explode STR ''x'' \<noteq> []"
+      proof 
+        assume "literal.explode STR ''x'' = []"
+        hence "literal.explode STR ''x'' = literal.explode STR ''''"
+          using literal.explode_inject zero_literal.rep_eq by auto
+        thus False using literal.explode_inject by auto
+      qed
+      hence "x < x + STR ''x''"
+        apply (subst less_literal.rep_eq)
+        apply (subst plus_literal.rep_eq)
+        apply (rule ord.lexordp_append_rightI)
+        by blast
+      hence "\<exists>z. x < z" by blast
+    }
+    thus "proper_interval (Some x) None = (\<exists>z. x < z)" by force
+  qed
+  show "\<And>x y::String.literal. proper_interval (Some x) (Some y) = (\<exists>z>x. z < y)"
+  proof -
+    fix x y::String.literal
+    {
+      assume "proper_interval (Some x) (Some y)" 
+      hence undefined unfolding proper_interval_literal.simps
+      have "\<exists>z>x. z < y" sorry
+    }
+    moreover 
+    {
+      assume "\<exists>z>x. z < y"
+      have "proper_interval (Some x) (Some y)" sorry
+    }
+    ultimately
+    show "proper_interval (Some x) (Some y) = (\<exists>z>x. z < y)" by blast
+  qed
+qed
+end
+
+
+value "STR '''' < STR ''a''"
+
+instantiation predicate :: proper_interval
+begin
+fun proper_interval_predicate::"predicate option \<Rightarrow> predicate option \<Rightarrow> bool" where
+"proper_interval_predicate None None = True" |
+"proper_interval_predicate (Some p) None = undefined" |
+"proper_interval_predicate None (Some p) = undefined" |
+"proper_interval_predicate (Some p) (Some q) = undefined"
+end
+
+instantiation predicate :: cproper_interval
+begin
+  
+end
+
+print_derives
+
+lemmas ground_ast_problem_code =
+  ground_ast_problem_defs.at_start_spec.simps
+  ground_ast_problem_defs.at_end_spec.simps
+  ground_ast_problem_defs.actions_spec_def
+  ground_ast_problem_defs.mutex_snap_action'_def
+  ground_ast_problem_defs.int_clocks_spec'_def
+  ground_ast_problem_defs.start_edge_spec'_def
+  ground_ast_problem_defs.edge_2_spec'_def
+  ground_ast_problem_defs.edge_3_spec'_def
+  ground_ast_problem_defs.instant_trans_edge_spec'_def
+  ground_ast_problem_defs.action_to_automaton_spec'_def
+  ground_ast_problem_defs.init_spec'_def
+  ground_ast_problem_defs.main_auto_init_edge_spec'_def
+  ground_ast_problem_defs.main_auto_goal_edge_spec'_def
+  ground_ast_problem_defs.main_auto_spec'_def
+  ground_ast_problem_defs.automata_spec'_def
+
+declare ground_ast_problem_code[code]
+
 
 context ground_ast_problem
 begin
-  subsection \<open>Now, we will refine these lemmas. Checking list intersection is inefficient
-  for all actions. We do not need to, because we have proven that actions only refer to propositions
+
+subsection \<open>Refinement to monadic code\<close>
+
+text \<open>Some constants need executable copies\<close>
+
+(* tp_nta_reduction_spec.planning_loc, tp_nta_reduction_spec.set_prop_ab, tp_nta_reduction_spec.acts_active, tp_nta_reduction_spec.init_loc *)
+
+lemma prop_to_var_refine: 
+  "abstr_model_checking.reduction_ref_impl.prop_to_var \<equiv> prop_to_var_impl predicate.name"
+  unfolding abstr_model_checking.reduction_ref_impl.prop_to_var_def
+  unfolding prop_to_var_impl_def prop_to_name_spec_def
+  by argo
+
+lemma prop_to_lock_refine: 
+  "abstr_model_checking.reduction_ref_impl.prop_to_lock \<equiv> prop_to_lock_impl predicate.name"
+  unfolding abstr_model_checking.reduction_ref_impl.prop_to_lock_def
+  unfolding prop_to_lock_impl_def prop_to_name_spec_def
+  by argo
+
+lemma acts_active_refine:
+  "abstr_model_checking.reduction_ref_impl.acts_active = acts_active_impl"
+  unfolding abstr_model_checking.reduction_ref_impl.acts_active_def
+  unfolding acts_active_impl_def
+  ..
+
+lemma planning_lock_refine:
+  "abstr_model_checking.reduction_ref_impl.planning_lock = planning_lock_impl"
+  unfolding abstr_model_checking.reduction_ref_impl.planning_lock_def
+  unfolding planning_lock_impl_def ..
+
+lemma act_to_start_clock_refine:
+  "abstr_model_checking.reduction_ref_impl.act_to_start_clock = act_to_start_clock_impl ast_action_schema.name"
+  unfolding abstr_model_checking.reduction_ref_impl.act_to_start_clock_def
+  unfolding act_to_name_spec_def
+  unfolding act_to_start_clock_impl_def
+  ..
+
+lemma act_to_end_clock_refine:
+  "abstr_model_checking.reduction_ref_impl.act_to_end_clock = act_to_end_clock_impl ast_action_schema.name"
+  unfolding abstr_model_checking.reduction_ref_impl.act_to_end_clock_def
+  unfolding act_to_name_spec_def
+  unfolding act_to_end_clock_impl_def
+  ..
+
+lemma off_loc_refine:
+  "abstr_model_checking.reduction_ref_impl.off_loc = off_loc_impl"
+  unfolding abstr_model_checking.reduction_ref_impl.off_loc_def
+  unfolding off_loc_impl_def
+  ..
+
+lemma starting_loc_refine:
+  "abstr_model_checking.reduction_ref_impl.starting_loc = starting_loc_impl"
+  unfolding abstr_model_checking.reduction_ref_impl.starting_loc_def
+  unfolding starting_loc_impl_def
+  ..
+
+lemma running_loc_refine:
+  "abstr_model_checking.reduction_ref_impl.running_loc = running_loc_impl"
+  unfolding abstr_model_checking.reduction_ref_impl.running_loc_def
+  unfolding running_loc_impl_def
+  ..
+
+lemma ending_loc_refine:
+  "abstr_model_checking.reduction_ref_impl.ending_loc = ending_loc_impl"
+  unfolding abstr_model_checking.reduction_ref_impl.ending_loc_def
+  unfolding ending_loc_impl_def
+  ..
+
+lemma init_loc_refine:
+  "abstr_model_checking.reduction_ref_impl.init_loc = init_loc_impl"
+  unfolding abstr_model_checking.reduction_ref_impl.init_loc_def
+  unfolding init_loc_impl_def
+  ..
+
+lemma planning_loc_refine:
+  "abstr_model_checking.reduction_ref_impl.planning_loc = planning_loc_impl"
+  unfolding abstr_model_checking.reduction_ref_impl.planning_loc_def
+  unfolding planning_loc_impl_def
+  ..
+
+lemma goal_loc_refine:
+  "abstr_model_checking.reduction_ref_impl.goal_loc = goal_loc_impl"
+  unfolding abstr_model_checking.reduction_ref_impl.goal_loc_def
+  unfolding goal_loc_impl_def
+  ..
+
+lemma set_prop_ab_refine:
+  "abstr_model_checking.reduction_ref_impl.set_prop_ab n = (set_var n) o (prop_to_var_impl predicate.name)"
+  unfolding abstr_model_checking.reduction_ref_impl.set_prop_ab_def
+  unfolding prop_to_var_refine
+  ..
+
+lemma is_prop_ab_refine:
+  "abstr_model_checking.reduction_ref_impl.is_prop_ab n = (var_is n) o (prop_to_var_impl predicate.name)"
+  unfolding abstr_model_checking.reduction_ref_impl.is_prop_ab_def
+  unfolding prop_to_var_refine
+  ..
+
+lemma inc_prop_ab_refine:
+  "abstr_model_checking.reduction_ref_impl.inc_prop_ab n = (inc_var n) o (prop_to_var_impl predicate.name)"
+  unfolding abstr_model_checking.reduction_ref_impl.inc_prop_ab_def
+  unfolding prop_to_var_refine
+  ..
+
+lemma set_prop_lock_ab_refine:
+  "abstr_model_checking.reduction_ref_impl.set_prop_lock_ab n = (set_var n) o (prop_to_lock_impl predicate.name)"
+  unfolding abstr_model_checking.reduction_ref_impl.set_prop_lock_ab_def
+  unfolding prop_to_lock_refine
+  ..
+
+lemma is_prop_lock_ab_refine:
+  "abstr_model_checking.reduction_ref_impl.is_prop_lock_ab n = (var_is n) o (prop_to_lock_impl predicate.name)"
+  unfolding abstr_model_checking.reduction_ref_impl.is_prop_lock_ab_def
+  unfolding prop_to_lock_refine
+  ..
+
+lemma inc_prop_lock_ab_refine:
+  "abstr_model_checking.reduction_ref_impl.inc_prop_lock_ab n = (inc_var n) o (prop_to_lock_impl predicate.name)"
+  unfolding abstr_model_checking.reduction_ref_impl.inc_prop_lock_ab_def
+  unfolding prop_to_lock_refine
+  ..
+
+lemma lower_spec_refine:
+  "lower_spec = lower_spec_impl"
+  apply (intro ext)
+  subgoal for x
+    apply (cases x)
+    by simp+
+  done
+
+lemma upper_spec_refine:
+  "upper_spec = upper_spec_impl"
+  apply (intro ext)
+  subgoal for x
+    apply (cases x)
+    by simp+
+  done
+
+schematic_goal l_dur_spec_refine:
+  "abstr_model_checking.reduction_ref_impl.l_dur_spec = l_dur_spec_impl"
+  apply (intro ext)
+  unfolding abstr_model_checking.reduction_ref_impl.l_dur_spec_def
+  unfolding lower_spec_refine
+  unfolding act_to_start_clock_refine
+  unfolding l_dur_spec_impl_def
+  ..
+
+schematic_goal u_dur_spec_refine:
+  "abstr_model_checking.reduction_ref_impl.u_dur_spec = u_dur_spec_impl"
+  apply (intro ext)
+  unfolding abstr_model_checking.reduction_ref_impl.u_dur_spec_def
+  unfolding upper_spec_refine
+  unfolding act_to_start_clock_refine
+  unfolding u_dur_spec_impl_def
+  ..
+
+
+
+text \<open>Now, we will refine these lemmas. Checking list intersection is inefficient
+  for all actions. We do not need to, because we have proven that actions only refer to 
+  propositions (predicates without arguments)
   at the level of PDDL.\<close>
 lemma pre_imp_restr_equiv_pre_imp:
   assumes "a \<in> AtStart ` set actions_spec \<union> AtEnd ` set actions_spec"
@@ -86,8 +654,15 @@ proof -
     by (force simp: filter_id_conv)
 qed
 
-definition "mutex_snap_action' a b = 
-  action_defs.mutex_snap_action (\<lambda>a. set (imp_defs.rat_impl.pre_imp_list a)) (\<lambda>a. set (imp_defs.rat_impl.add_imp_list a)) (\<lambda>a. set (imp_defs.rat_impl.del_imp_list a)) a b"
+lemma over_all_restr_equiv_over_all:
+  assumes "a \<in> set actions_spec"
+  shows "imp_defs.rat_impl.over_all_restr_list a = over_all_spec a"
+proof -
+  have "set (over_all_spec a) \<subseteq> set props_spec"
+    using over_all_in_props assms by simp
+  thus ?thesis unfolding imp_defs.rat_impl.over_all_restr_list_def
+    by (force simp: filter_id_conv)
+qed
 
 
 lemma mutex_snap_action_refine:
@@ -100,11 +675,6 @@ lemma mutex_snap_action_refine:
   unfolding comp_def apply (subst pre_imp_restr_equiv_pre_imp, use assms in blast)+
   apply (subst action_defs.mutex_snap_action_def[symmetric])
   by simp
-
-definition "int_clocks_spec' a =
-    map abstr_model_checking.reduction_ref_impl.act_to_start_clock (filter (\<lambda>b. mutex_snap_action' a (AtStart b)) actions_spec) 
-  @ map abstr_model_checking.reduction_ref_impl.act_to_end_clock (filter (\<lambda>aa. mutex_snap_action' a (AtEnd aa)) actions_spec)"
-  
 
 lemma int_clocks_spec_refine:
   assumes "a \<in> AtStart ` set actions_spec \<union> AtEnd ` set actions_spec"
@@ -125,69 +695,88 @@ proof -
   show ?thesis
     unfolding abstr_model_checking.reduction_ref_impl.int_clocks_spec_def Let_def
     unfolding 1 2 int_clocks_spec'_def
+    unfolding act_to_start_clock_refine
+    unfolding act_to_end_clock_refine
     by blast
 qed
-
-definition "start_edge_spec' a = 
-(let start_snap = AtStart a; guard = map (\<lambda>x. acconstraint.GT x 0) (int_clocks_spec' start_snap) @ map (\<lambda>x. acconstraint.GE x 0) (int_clocks_spec' start_snap);
-         not_locked_check = map (abstr_model_checking.reduction_ref_impl.is_prop_lock_ab 0) (filter (\<lambda>p. p \<notin> set (imp_defs.rat_impl.add_imp_list start_snap)) (imp_defs.rat_impl.del_imp_list start_snap)); pre_check = map (abstr_model_checking.reduction_ref_impl.is_prop_ab 1) (imp_defs.rat_impl.pre_imp_restr_list start_snap);
-         var_check = abstr_model_checking.reduction_ref_impl.bexp_and_all (not_locked_check @ pre_check); add_upds = map (abstr_model_checking.reduction_ref_impl.set_prop_ab 1) (imp_defs.rat_impl.add_imp_list start_snap); del_upds = map (abstr_model_checking.reduction_ref_impl.set_prop_ab 0) (imp_defs.rat_impl.del_imp_list start_snap);
-         upds = (abstr_model_checking.reduction_ref_impl.acts_active, binop plus_int (var abstr_model_checking.reduction_ref_impl.acts_active) (exp.const 1)) # del_upds @ add_upds; resets = [abstr_model_checking.reduction_ref_impl.act_to_start_clock a]
-     in (abstr_model_checking.reduction_ref_impl.off_loc, var_check, guard, Sil STR '''', upds, resets, abstr_model_checking.reduction_ref_impl.starting_loc))"
 
 lemma start_edge_spec_refine:
   assumes "a \<in> set actions_spec"
   shows "abstr_model_checking.reduction_ref_impl.start_edge_spec a = start_edge_spec' a" 
   unfolding start_edge_spec'_def
   unfolding abstr_model_checking.reduction_ref_impl.start_edge_spec_def
-  using int_clocks_spec_refine assms
+  unfolding is_prop_lock_ab_refine
+  unfolding is_prop_ab_refine
+  unfolding set_prop_ab_refine
+  unfolding acts_active_refine
+  unfolding off_loc_refine starting_loc_refine
+  unfolding act_to_start_clock_refine
+  using int_clocks_spec_refine assms pre_imp_restr_equiv_pre_imp
   by simp
 
-definition "edge_3_spec' a =
-(let end_snap = AtEnd a; int_clocks = map (\<lambda>x. acconstraint.GT x 0) (int_clocks_spec' end_snap) @ map (\<lambda>x. acconstraint.GE x 0) (int_clocks_spec' end_snap); guard = abstr_model_checking.reduction_ref_impl.l_dur_spec a @ abstr_model_checking.reduction_ref_impl.u_dur_spec a @ int_clocks;
-         upds = map (abstr_model_checking.reduction_ref_impl.inc_prop_lock_ab (- 1)) (imp_defs.rat_impl.over_all_restr_list a); resets = [abstr_model_checking.reduction_ref_impl.act_to_end_clock a]
-     in (abstr_model_checking.reduction_ref_impl.running_loc, bexp.true, guard, Sil STR '''', upds, resets, abstr_model_checking.reduction_ref_impl.ending_loc))"
+
+lemma edge_2_spec_refine:
+  assumes "a \<in> set actions_spec"
+  shows "abstr_model_checking.reduction_ref_impl.edge_2_spec a = edge_2_spec' a" 
+  unfolding abstr_model_checking.reduction_ref_impl.edge_2_spec_def 
+  unfolding is_prop_ab_refine
+  unfolding inc_prop_lock_ab_refine
+  unfolding starting_loc_refine running_loc_refine
+  unfolding edge_2_spec'_def
+  using over_all_restr_equiv_over_all assms
+  by simp
 
 lemma edge_3_spec_refine:
   assumes "a \<in> set actions_spec"
   shows "abstr_model_checking.reduction_ref_impl.edge_3_spec a = edge_3_spec' a" 
   unfolding abstr_model_checking.reduction_ref_impl.edge_3_spec_def
   unfolding edge_3_spec'_def
-  using int_clocks_spec_refine assms
+  unfolding running_loc_refine
+  unfolding ending_loc_refine
+  unfolding act_to_end_clock_refine
+  unfolding inc_prop_lock_ab_refine
+  unfolding l_dur_spec_refine u_dur_spec_refine
+  using int_clocks_spec_refine assms over_all_restr_equiv_over_all
   by simp
 
-definition "instant_trans_edge_spec' a =
-(let end_snap = AtEnd a; start_snap = AtStart a; int_clocks = map (\<lambda>x. acconstraint.GT x 0) (int_clocks_spec' end_snap) @ map (\<lambda>x. acconstraint.GE x 0) (int_clocks_spec' end_snap); guard = abstr_model_checking.reduction_ref_impl.l_dur_spec a @ abstr_model_checking.reduction_ref_impl.u_dur_spec a @ int_clocks;
-         resets = [abstr_model_checking.reduction_ref_impl.act_to_end_clock a]
-     in (abstr_model_checking.reduction_ref_impl.starting_loc, bexp.true, guard, Sil STR '''', [], resets, abstr_model_checking.reduction_ref_impl.ending_loc))"
+
+lemma end_edge_spec_refine:
+  assumes "a \<in> set actions_spec"
+  shows "abstr_model_checking.reduction_ref_impl.end_edge_spec a = end_edge_spec' a"
+  unfolding abstr_model_checking.reduction_ref_impl.end_edge_spec_def
+  unfolding ending_loc_refine off_loc_refine
+  unfolding is_prop_ab_refine
+  unfolding is_prop_lock_ab_refine
+  unfolding set_prop_ab_refine
+  unfolding acts_active_refine
+  unfolding end_edge_spec'_def
+  using pre_imp_restr_equiv_pre_imp assms
+  by auto
+
 
 lemma instant_trans_edge_spec_refine:
   assumes "a \<in> set actions_spec"
   shows "abstr_model_checking.reduction_ref_impl.instant_trans_edge_spec a = instant_trans_edge_spec' a" 
   unfolding abstr_model_checking.reduction_ref_impl.instant_trans_edge_spec_def
   unfolding instant_trans_edge_spec'_def
+  unfolding starting_loc_refine ending_loc_refine
+  unfolding l_dur_spec_refine u_dur_spec_refine
+  unfolding act_to_end_clock_refine
   using int_clocks_spec_refine assms
   by simp
 
-definition "action_to_automaton_spec' a =
-(let committed_locs = []; 
-  urgent_locs = [abstr_model_checking.reduction_ref_impl.starting_loc, abstr_model_checking.reduction_ref_impl.ending_loc]; 
-  edges = [start_edge_spec' a, abstr_model_checking.reduction_ref_impl.edge_2_spec a, edge_3_spec' a, abstr_model_checking.reduction_ref_impl.end_edge_spec a, instant_trans_edge_spec' a];
-  invs = []
-in (committed_locs, urgent_locs, edges, invs))"
 
 lemma action_to_automaton_spec_refine:
   assumes "a \<in> set actions_spec"
   shows "abstr_model_checking.reduction_ref_impl.action_to_automaton_spec a = action_to_automaton_spec' a"
   unfolding abstr_model_checking.reduction_ref_impl.action_to_automaton_spec_def
   unfolding action_to_automaton_spec'_def
-  using start_edge_spec_refine edge_3_spec_refine instant_trans_edge_spec_refine assms by simp
+  unfolding starting_loc_refine ending_loc_refine
+  using start_edge_spec_refine edge_2_spec_refine edge_3_spec_refine end_edge_spec_refine instant_trans_edge_spec_refine assms
+  by simp
 
 
-thm abstr_model_checking.reduction_ref_impl.main_auto_spec_def
-thm abstr_model_checking.reduction_ref_impl.main_auto_init_edge_spec_def
-
-definition "init_spec' = (map to_predicate (filter is_predAtom (init P)))"
+text \<open>Now we provide an equivalent definition of the main automaton.\<close>
 
 
 lemma filter_props_init:
@@ -209,72 +798,46 @@ lemma filter_props_goal:
   using goal_in_props filter_id_conv by fast
 
   
-(* tp_nta_reduction_spec.planning_lock, tp_nta_reduction_spec.planning_loc, tp_nta_reduction_spec.set_prop_ab, tp_nta_reduction_spec.acts_active, tp_nta_reduction_spec.init_loc *)
-
-definition "planning_lock' = STR ''planning_lock''"
-
-lemma planning_lock_refine:
-  "abstr_model_checking.reduction_ref_impl.planning_lock = planning_lock'"
-  unfolding abstr_model_checking.reduction_ref_impl.planning_lock_def
-  unfolding planning_lock'_def ..
-
-definition "main_auto_init_edge_spec' \<equiv>
-(let can_start = Simple_Expressions.bexp.eq (var planning_lock') (exp.const 0); permit_planning = (abstr_model_checking.reduction_ref_impl.planning_lock, exp.const 1); set_active = (abstr_model_checking.reduction_ref_impl.acts_active, exp.const 0);
-         set_props = map (abstr_model_checking.reduction_ref_impl.set_prop_ab 1) init_spec'; upds = permit_planning # set_active # set_props
-     in (abstr_model_checking.reduction_ref_impl.init_loc, can_start, [], Sil STR '''', upds, [], abstr_model_checking.reduction_ref_impl.planning_loc))
-"
-
 lemma main_auto_init_edge_spec_refine:
   "abstr_model_checking.reduction_ref_impl.main_auto_init_edge_spec = main_auto_init_edge_spec'"
   unfolding abstr_model_checking.reduction_ref_impl.main_auto_init_edge_spec_def
   unfolding main_auto_init_edge_spec'_def
-  unfolding filter_props_init 
+  unfolding filter_props_init planning_lock_refine
+  unfolding planning_loc_refine
+  unfolding init_loc_refine
+  unfolding acts_active_refine
+  unfolding set_prop_ab_refine
   ..
-
-definition main_auto_goal_edge_spec'::"nat \<times>
-   (String.literal, int) Simple_Expressions.bexp \<times>
-   (String.literal, int) acconstraint list \<times>
-   String.literal act \<times>
-   (String.literal \<times> (String.literal, int) exp) list \<times> String.literal list \<times> nat" where
-"main_auto_goal_edge_spec' \<equiv>
-(let can_end = [Simple_Expressions.bexp.eq (var abstr_model_checking.reduction_ref_impl.planning_lock) (exp.const 1), Simple_Expressions.bexp.eq (var abstr_model_checking.reduction_ref_impl.acts_active) (exp.const 0)]; 
-  goal_sat = map (abstr_model_checking.reduction_ref_impl.is_prop_ab 1) goal_spec;
-  cond = abstr_model_checking.reduction_ref_impl.bexp_and_all (can_end @ goal_sat); 
-  lock_plan = (abstr_model_checking.reduction_ref_impl.planning_lock, exp.const 2)
-in (abstr_model_checking.reduction_ref_impl.planning_loc, cond, [], Sil STR '''', [lock_plan], [], abstr_model_checking.reduction_ref_impl.goal_loc))
-"
 
 lemma main_auto_goal_edge_spec_refine:
   "abstr_model_checking.reduction_ref_impl.main_auto_goal_edge_spec = main_auto_goal_edge_spec'"
   unfolding abstr_model_checking.reduction_ref_impl.main_auto_goal_edge_spec_def
   unfolding main_auto_goal_edge_spec'_def
   unfolding filter_props_goal
+  unfolding planning_loc_refine
+  unfolding goal_loc_refine
+  unfolding acts_active_refine
+  unfolding planning_lock_refine
+  unfolding is_prop_ab_refine
   ..
 
-definition main_auto_spec'::"nat list \<times>
-   nat list \<times>
-   (nat \<times>
-    (String.literal, int) Simple_Expressions.bexp \<times>
-    (String.literal, int) acconstraint list \<times>
-    String.literal act \<times>
-    (String.literal \<times> (String.literal, int) exp) list \<times>
-    String.literal list \<times> nat) list \<times>
-   (nat \<times> (String.literal, int) acconstraint list) list" where
-"main_auto_spec' \<equiv>
-(let committed_locs = []; 
-  urgent_locs = [abstr_model_checking.reduction_ref_impl.init_loc, abstr_model_checking.reduction_ref_impl.goal_loc]; 
-  edges = [main_auto_init_edge_spec', main_auto_goal_edge_spec', abstr_model_checking.reduction_ref_impl.main_auto_loop_spec]; 
-  invs = [] 
-in (committed_locs, urgent_locs, edges, invs))"
+lemma main_auto_loop_spec_refine:
+  "abstr_model_checking.reduction_ref_impl.main_auto_loop_spec = main_auto_loop_spec_impl"
+  unfolding abstr_model_checking.reduction_ref_impl.main_auto_loop_spec_def
+  unfolding main_auto_loop_spec_impl_def
+  unfolding goal_loc_refine ..
 
 lemma main_auto_spec_refine:
   "abstr_model_checking.reduction_ref_impl.main_auto_spec = main_auto_spec'"
   unfolding abstr_model_checking.reduction_ref_impl.main_auto_spec_def
   unfolding main_auto_spec'_def
   unfolding main_auto_init_edge_spec_refine main_auto_goal_edge_spec_refine
+  unfolding main_auto_loop_spec_refine
+  unfolding init_loc_refine goal_loc_refine
   ..
 
-definition "automata_spec' = main_auto_spec' # map action_to_automaton_spec' actions_spec"
+
+text \<open>Finally we can provide another definition of the entire network\<close>
 
 lemma automata_spec_refine:
   shows "abstr_model_checking.reduction_ref_impl.automata_spec = automata_spec'"
@@ -283,97 +846,45 @@ lemma automata_spec_refine:
   using action_to_automaton_spec_refine main_auto_spec_refine by simp
 
 end
-thm ground_ast_problem.action_to_automaton_spec'_def
 
-thm ground_ast_problem.automata_spec'_def
-
-thm ground_ast_problem_defs.init_spec_def
-
-fun to_predicateM where
-"to_predicateM (Atom (predAtm x _)) = Error_Monad.return x" |
-"to_predicateM x = Error_Monad.error (ERRS ''Not an atomic predicate formula'')"
-
-lemma to_predicateM_return_if[return_if]: 
-  "is_predAtom x \<Longrightarrow> ((to_predicateM x = Inr y) \<longleftrightarrow> ground_ast_problem_defs.to_predicate x = y)"
-  apply (induction x arbitrary: y rule: ground_ast_problem_defs.to_predicate.induct)
-  subgoal apply (subst to_predicateM.simps)
-    apply (subst ground_ast_problem_defs.to_predicate.simps)
-    by blast
-  by simp+
+text \<open>We will now refine the code to monadic implementations. \<close>
 
 definition init_specM::"ast_problem \<Rightarrow> (unit \<Rightarrow> char list \<Rightarrow> char list) + _" where
 "init_specM P \<equiv> do {
-  mapM to_predicateM (filter is_predAtom (init P))
+  Error_Monad.return (map to_predicate (filter is_predAtom (init P)))
 }"
 
 
-lemma mapM_return_iff[return_iff]: "mapM f xs = Inr ys \<longleftrightarrow> list_all2 (\<lambda>x y. f x = Inr y) xs ys"
-proof (rule iffI)
-  assume a: "mapM f xs = Inr ys"
-  have len: "length xs = length ys" using a mapM_return by fastforce
-  show "list_all2 (\<lambda>x y. f x = Inr y) xs ys"
-  proof (rule list_all2_all_nthI[OF len])
-    fix n
-    assume n: "n < length xs" 
-    have ys: "ys = map (projr \<circ> f) xs" 
-      and xs_r: "(\<forall>x\<in>set xs. \<forall>e. f x \<noteq> Inl e)" using a[THEN mapM_return] by blast+
-    have obtain r where
-        xs_n_inr: "f (xs ! n) = Inr r" using xs_r n apply (cases "f (xs ! n)") by auto
-    have "ys ! n = r" using xs_n_inr ys unfolding comp_def using n by simp
-    thus "f (xs ! n) = Inr (ys ! n)" using xs_n_inr by simp
-  qed
-next
-  assume a: "list_all2 (\<lambda>x y. f x = Inr y) xs ys"
-  thus "mapM f xs = Inr ys"
-    by (induction rule: list_all2_induct) auto
-qed
-
-
-lemma list_all2_return_if[return_if]:
-  assumes "list_all P xs"
-      and "\<And>x y. P x \<Longrightarrow> fM x = Inr y \<longleftrightarrow> f x = y"
-    shows "list_all2 (\<lambda>x y. fM x = Inr y) xs ys = (ys = map f xs)"
-  unfolding list_all2_conv_all_nth
-proof (intro iffI strip conjI; (elim conjE)?)
-  assume len: "length xs = length ys" 
-    and i: "\<forall>i<length xs. fM (xs ! i) = Inr (ys ! i)"
-  have nth_eq: "\<forall>i < length xs. ys ! i = f (xs ! i)" using i assms unfolding list_all_iff by simp
-  show "ys = map f xs" apply (subst list_eq_iff_nth_eq)
-    using len nth_eq by auto 
-next
-  show "ys = map f xs \<Longrightarrow> length xs = length ys" by simp
-next
-  fix i
-  assume ys: "ys = map f xs"
-    and i: "i < length xs"
-  show "fM (xs ! i) = Inr (ys ! i)"
-    using assms ys i unfolding list_all_iff by auto
-qed
-
-lemma init_specM_return_if[return_if]:
+lemma init_specM_return_if:
   assumes "ground_ast_problem P" 
   shows "(init_specM P = Inr x \<longleftrightarrow> x = ground_ast_problem.init_spec' P)"
-  unfolding init_specM_def 
-proof -
-  show "(mapM to_predicateM (filter is_predAtom (init P)) = Inr x) = (x = ground_ast_problem.init_spec' P)"
-    apply (subst mapM_return_iff)
-    apply (subst ground_ast_problem.init_spec'_def)
-     apply (rule assms)
-    apply (rule list_all2_return_if[where P = is_predAtom])
-    unfolding list_all_iff using to_predicateM_return_if by auto
-qed
+  unfolding init_specM_def
+  apply (subst ground_ast_problem.init_spec'_def)
+  using assms by blast+
+
+value "ground_ast_problem_defs.init_spec' example_problem"
+
+
+definition goal_specM::"ast_problem \<Rightarrow> (unit \<Rightarrow> string \<Rightarrow> string) + _" where
+"goal_specM P \<equiv> do {
+  Error_Monad.return (remdups (map to_predicate (to_literals (goal P))))
+}"
+
+
+lemma goal_specM_return_if:
+  assumes "ground_ast_problem P"
+  shows "goal_specM P = Inr x \<longleftrightarrow> x = ground_ast_problem_defs.goal_spec P"
+  unfolding goal_specM_def
+  using assms ground_ast_problem_defs.goal_spec_def
+  by fastforce
   
-  
-(* tp_nta_reduction_spec.planning_lock, tp_nta_reduction_spec.planning_loc, tp_nta_reduction_spec.set_prop_ab, tp_nta_reduction_spec.acts_active, tp_nta_reduction_spec.init_loc *)
 
 lemma [code]: "ground_ast_problem_defs.prop_to_name_spec = predicate.name"
   unfolding ground_ast_problem_defs.prop_to_name_spec_def by simp
 
-thm tp_nta_reduction_spec.planning_loc_def
 
-definition "planning_lock_specM = "
-
-definition main_auto_init_edge_specM::"_ \<Rightarrow> (unit \<Rightarrow> char list \<Rightarrow> char list) + 
+definition main_auto_init_edge_specM::"_ \<Rightarrow> 
+  (unit \<Rightarrow> char list \<Rightarrow> char list) + 
   (nat \<times>
     (String.literal, int) Simple_Expressions.bexp \<times>
     (String.literal, int) acconstraint list \<times>
@@ -382,34 +893,126 @@ definition main_auto_init_edge_specM::"_ \<Rightarrow> (unit \<Rightarrow> char 
     String.literal list \<times> nat)" where
 "main_auto_init_edge_specM P \<equiv> do {
 init \<leftarrow> init_specM P;
-let can_start = Simple_Expressions.bexp.eq (var tp_nta_reduction_spec.planning_lock) (exp.const 0);
-let permit_planning = (tp_nta_reduction_spec.planning_lock, exp.const 1); 
-let set_active = (tp_nta_reduction_spec.acts_active, exp.const 0);
-let set_props = map (tp_nta_reduction_spec.set_prop_ab ground_ast_problem_defs.prop_to_name_spec 1) init; 
+let can_start = var_is 0 planning_lock_impl;
+let permit_planning = set_var 1 planning_lock_impl; 
+let set_active = set_var 0 acts_active_impl;
+let set_props = map ((set_var 1 \<circ>\<circ> prop_to_var_impl) predicate.name) init; 
 let upds = permit_planning # set_active # set_props;
- Error_Monad.return (tp_nta_reduction_spec.init_loc, can_start, [], Sil STR '''', upds, [], tp_nta_reduction_spec.planning_loc)
+ Error_Monad.return (init_loc_impl, can_start, [], Sil STR '''', upds, [], planning_loc_impl)
 }"
 
-value "main_auto_init_edge_specM example_problem" 
+value "main_auto_init_edge_specM example_problem"
 
-thm ground_ast_problem.main_auto_init_edge_spec'_def[no_vars]
+lemma main_auto_init_edge_specM_return_if:
+  assumes "ground_ast_problem P"
+  shows "main_auto_init_edge_specM P = Inr x \<longleftrightarrow> x = ground_ast_problem.main_auto_init_edge_spec' P"
+  unfolding main_auto_init_edge_specM_def
+  apply (subst ground_ast_problem.main_auto_init_edge_spec'_def[OF assms])
+  unfolding init_specM_return_if[OF assms] return_iff 
+  by auto
+
+definition main_auto_goal_edge_specM::"_ \<Rightarrow> (unit \<Rightarrow> char list \<Rightarrow> char list) + 
+  (nat \<times>
+    (String.literal, int) Simple_Expressions.bexp \<times>
+    (String.literal, int) acconstraint list \<times>
+    String.literal act \<times>
+    (String.literal \<times> (String.literal, int) exp) list \<times>
+    String.literal list \<times> nat)" where
+"main_auto_goal_edge_specM P \<equiv> do {
+goal' \<leftarrow> goal_specM P;
+let can_end = [var_is 1 planning_lock_impl, var_is 0 acts_active_impl]; 
+let goal_sat = map ((var_is 1 \<circ>\<circ> prop_to_var_impl) predicate.name) goal';
+let cond = bexp_and_all (can_end @ goal_sat); 
+let lock_plan = (planning_lock_impl, exp.const 2);
+Error_Monad.return (planning_loc_impl, cond, [], Sil STR '''', [lock_plan], [], goal_loc_impl)
+}"
+
+value "main_auto_goal_edge_specM example_problem"
+
+lemma main_auto_goal_edge_specM_return_if:
+  assumes "ground_ast_problem P"
+  shows "main_auto_goal_edge_specM P = Inr x \<longleftrightarrow> x = ground_ast_problem.main_auto_goal_edge_spec' P"
+  unfolding main_auto_goal_edge_specM_def
+  apply (subst ground_ast_problem.main_auto_goal_edge_spec'_def[OF assms])
+  unfolding goal_specM_return_if[OF assms] return_iff 
+  by auto
 
 
-definition "main_auto_specM P \<equiv> do {
-let committed_locs = []; 
-  urgent_locs = [tp_nta_reduction_spec.init_loc, tp_nta_reduction_spec.goal_loc]; 
-  edges = [ground_ast_problem.main_auto_init_edge_spec' P, ground_ast_problem.main_auto_goal_edge_spec' P, tp_nta_reduction_spec.main_auto_loop_spec]; 
-  invs = [] 
-in 
+thm temp_planning_problem_list_defs.add_imp_list_def
+
+find_theorems name: "start_edge_spec'"
+
+(* (unit \<Rightarrow> char list \<Rightarrow> char list) + 
+  (nat \<times>
+    (String.literal, int) Simple_Expressions.bexp \<times>
+    (String.literal, int) acconstraint list \<times>
+    String.literal act \<times>
+    (String.literal \<times> (String.literal, int) exp) list \<times>
+    String.literal list \<times> nat)
+*)
+
+definition main_auto_specM::"_ \<Rightarrow> (unit \<Rightarrow> string \<Rightarrow> string) +
+  (nat list \<times>
+      nat list \<times>
+      (nat \<times>
+       (String.literal, int) Simple_Expressions.bexp \<times>
+       (String.literal, int) acconstraint list \<times>
+       String.literal act \<times>
+       (String.literal \<times> (String.literal, int) exp) list \<times>
+       String.literal list \<times> nat) list \<times>
+      (nat \<times> (String.literal, int) acconstraint list) list)" where
+"main_auto_specM P \<equiv> 
+do {
+  
+  init_edge \<leftarrow> main_auto_init_edge_specM P;
+  goal_edge \<leftarrow> main_auto_goal_edge_specM P;
+  let loop_edge = main_auto_loop_spec_impl;
+  let committed_locs = ([]::nat list); 
+  let urgent_locs = [init_loc_impl, goal_loc_impl];
+  let edges = [init_edge, goal_edge, loop_edge]; 
+  let invs = [];
   Error_Monad.return (committed_locs, urgent_locs, edges, invs)
 }"
 
 thm ground_ast_problem.main_auto_spec'_def
 
-value "ground_ast_problem.main_auto_spec' example_problem"
+value "main_auto_specM example_problem"
+
+lemma main_auto_specM_return_if:
+  assumes "ground_ast_problem P"
+  shows "main_auto_specM P = Inr x \<longleftrightarrow> x = ground_ast_problem.main_auto_spec' P"
+  unfolding main_auto_specM_def
+  unfolding ground_ast_problem.main_auto_spec'_def[OF assms]
+  by (auto simp: return_iff main_auto_init_edge_specM_return_if[OF assms] main_auto_goal_edge_specM_return_if[OF assms])
+
+text \<open>We have provided a monadic definition of the main automaton. Now, we will provide one for the 
+other automata.\<close>
+
+
+code_thms ground_ast_problem_defs.at_start_spec
+value "ground_ast_problem_defs.at_start_spec"
+
+find_theorems name: "ground_ast_problem.start_edge_spec'_def"
+
+definition start_edge_specM where
+"start_edge_specM P a \<equiv> do {
+let start_snap = AtStart a; 
+let guard = map (\<lambda>x. acconstraint.GT x 0) (ground_ast_problem_defs.int_clocks_spec' start_snap) @ map (\<lambda>x. acconstraint.GE x 0) (ground_ast_problem_defs.int_clocks_spec' start_snap);
+let not_locked_check = map ((var_is 0 \<circ>\<circ> prop_to_lock_impl) predicate.name) (filter (\<lambda>p. p \<notin> set (imp_defs.rat_impl.add_imp_list start_snap)) (imp_defs.rat_impl.del_imp_list start_snap)); 
+let pre_check = map ((var_is 1 \<circ>\<circ> prop_to_var_impl) predicate.name) (imp_defs.rat_impl.pre_imp_list start_snap);
+let var_check = bexp_and_all (not_locked_check @ pre_check); 
+let add_upds = map ((set_var 1 \<circ>\<circ> prop_to_var_impl) predicate.name) (imp_defs.rat_impl.add_imp_list start_snap); 
+let del_upds = map ((set_var 0 \<circ>\<circ> prop_to_var_impl) predicate.name) (imp_defs.rat_impl.del_imp_list start_snap);
+let upds = (inc_var 1 acts_active_impl) # del_upds @ add_upds; 
+let resets = [act_to_start_clock_impl ast_action_schema.name a];
+Error_Monad.return (off_loc_impl, var_check, guard, Sil STR '''', upds, resets, starting_loc_impl)
+}"
+
+
+value "ground_ast_problem_defs.automata_spec' example_problem"
 
 definition "automata_specM P \<equiv> do {
-  Error_Monad.return (ground_ast_problem.automata_spec' P)
+  Error_Monad.return (ground_ast_problem_defs.automata_spec' P)
 }"
 
 definition make_network where
