Ground_PDDL_Exec_Imp/Ground_PDDL_Problem_Code.thy
@@ -1,0 +1,80 @@
+theory Ground_PDDL_Problem_Code
+  imports Ground_PDDL_Problem_Defs
+begin
+
+(* fun at_start_spec::"ast_action_schema \<Rightarrow> ground_action" where
+"at_start_spec (Simple_Action_Schema n ps pre eff) = instantiate_action_schema (Simple_Action_Schema n ps pre eff) [] At_Start" |
+"at_start_spec (Durative_Action_Schema n ps d cond eff) = inst_snap_action (Durative_Action_Schema n ps d cond eff) [] At_Start"
+
+fun at_end_spec::"ast_action_schema \<Rightarrow> ground_action" where
+"at_end_spec (Simple_Action_Schema n ps pre eff) = ground_non_action n At_End" |
+"at_end_spec (Durative_Action_Schema n ps d cond eff) = inst_snap_action (Durative_Action_Schema n ps d cond eff) [] At_End"
+
+fun over_all_snap::"ast_action_schema \<Rightarrow> ground_action" where
+"over_all_snap (Simple_Action_Schema n ps pre eff) = 
+   ground_non_action n Over_All" |
+"over_all_snap (Durative_Action_Schema n ps d cond eff) = 
+  inst_snap_action (Durative_Action_Schema n ps d cond eff) [] Over_All"
+
+fun pre_spec::"ground_action \<Rightarrow> predicate list" where
+"pre_spec (Ground_Action n anno form eff) = 
+  form
+  |> to_literals
+  |> map to_predicate
+  |> remdups"
+
+fun over_all_spec::"ast_action_schema \<Rightarrow> predicate list" where
+"over_all_spec x =
+  x
+  |> over_all_snap
+  |> pre_spec"
+
+fun adds_spec::"ground_action \<Rightarrow> predicate list" where
+"adds_spec (Ground_Action n anno form eff) =
+  eff
+  |> ast_effect.adds
+  |> map to_predicate
+  |> remdups
+"
+
+fun dels_spec::"ground_action \<Rightarrow> predicate list" where
+"dels_spec (Ground_Action n anno form eff) =
+  eff
+  |> ast_effect.dels
+  |> map to_predicate
+  |> remdups
+"
+
+fun dc_to_lb::"term duration_constraint \<Rightarrow> rat lower_bound option" where
+"dc_to_lb No_Const = None" |
+"dc_to_lb (Time_Const duration_op.EQ x) = Some (lower_bound.GE x)" |
+"dc_to_lb (Time_Const duration_op.GEQ x) = Some (lower_bound.GE x)" |
+"dc_to_lb (Time_Const duration_op.LEQ x) = None"
+
+
+definition dc_list_lower::"term duration_constraint list \<Rightarrow> rat lower_bound option" where
+"dc_list_lower xs \<equiv> map dc_to_lb xs |> (\<lambda>xs. max_lb_opt xs None)" 
+
+
+fun dc_to_ub::"term duration_constraint \<Rightarrow> rat upper_bound option" where
+"dc_to_ub No_Const = None" |
+"dc_to_ub (Time_Const duration_op.EQ x) = Some (upper_bound.LE  x)" |
+"dc_to_ub (Time_Const duration_op.GEQ x) = None" |
+"dc_to_ub (Time_Const duration_op.LEQ x) = Some (upper_bound.LE x)"
+
+definition dc_list_upper::"term duration_constraint list \<Rightarrow> rat upper_bound option" where
+"dc_list_upper xs = map dc_to_ub xs |> (\<lambda>xs. min_ub_opt xs None)" 
+
+fun lower_spec::"ast_action_schema \<Rightarrow> _" where
+"lower_spec (Simple_Action_Schema n ps pre eff) = Some (lower_bound.GE 0)" | (* could also be None *)
+"lower_spec (Durative_Action_Schema n ps d cond eff) = map_option (map_lower_bound floor) (dc_list_lower d)"
+
+fun upper_spec::"ast_action_schema \<Rightarrow> _" where
+"upper_spec (Simple_Action_Schema n ps pre eff) = Some (upper_bound.LE 0)" | (* could also be None *)
+"upper_spec (Durative_Action_Schema n ps d cond eff) = map_option (map_upper_bound floor) (dc_list_upper d)"
+
+ *)
+
+
+ 
+end
